# part 3 A
(A x B) mod C = 1
## A

(1 x B) mod 9 = 1

1x1 mod9=1

(1 x 1) mod 9 = 1
## B
(5 x B) mod 9 = 1

5x1 mod9=5

5x2 mod9=1

(5 x 2) mod 9 = 1
## C
(7 x B) mod 9 = 1

7x1 mod9= 7

7x2 mod9= 5

7x3 mod9= 3

7x4 mod9= 1

(7 x 4) mod 9 = 1
## D
(16 x B) mod 9 = 1

16x1 mod9= 7

16x2 mod9= 5

16x3 mod9= 3

16x4 mod9= 1

(16 x 4) mod 9 = 1

# part 3 B
## A
(0 x B) mod 9 = 1

0x1 mod9= 0

0x2 mod9= 0

0x3 mod9= 0

0x4 mod9= 0

0x5 mod9= 0

0x6 mod9= 0

0x7 mod9= 0

0x8 mod9= 0
## B
(6 x B) mod 9 = 1

6x1 mod9= 6

6x2 mod9= 3

6x3 mod9= 0

6x4 mod9= 6

6x5 mod9= 3

6x6 mod9= 0

6x7 mod9= 6

6x8 mod9= 3
# C
(18 x B) mod 9 = 1

18x1 mod9= 0

18x2 mod9= 0

18x3 mod9= 0

18x4 mod9= 0

18x5 mod9= 0

18x6 mod9= 0

18x7 mod9= 0

18x8 mod9= 0
